ConstantPropagationAnalysis.v
@@ -1,55 +1,55 @@
 Require Import CSet Le.
 
 Require Import Plus Util AllInRel CSet.
-Require Import Val Var Env EnvTy IL Annotation Lattice DecSolve Analysis Filter.
+Require Import Val Var Env EnvTy IL Annotation Lattice DecSolve Analysis Filter Lattice.
 
 Require Import CMap.
-
-Definition Dom := option (Map [var, val]).
 
 Set Implicit Arguments.
 
 Open Scope map_scope.
 
-Definition join (v v' : option val) : option val :=
+Definition Dom := Map [var, withTop val].
+
+Definition join (v v' : option (withTop val)) : option (withTop val) :=
   match v, v' with
-    | Some v, Some v' => if [v = v'] then Some v else None
-    | _, _ => None
+    | Some (wTA v), Some (wTA v') => if [v = v'] then Some (wTA v) else Some Top
+    | Some (Top), _ => Some Top
+    | _, Some Top => Some Top
+    | Some (wTA v), _ => Some (wTA v)
+    | _, Some (wTA v) => Some (wTA v)
+    | None, None => None
   end.
 
-Definition joinDom (d d':Dom) : Dom :=
-  match d, d' with
-    | Some E, Some E' => Some (map2 join E E')
-    | Some E, _ => Some E
-    | _, Some E' => Some E'
-    | _, _ => None
-  end.
-
+Definition joinDom (d d':Dom) : Dom := map2 join d d'.
 
 Definition domain {X} `{OrderedType X} {Y} (d:Map [X, Y])
-: set X := fold (fun (k:X) _ (a:set X) => {k; a}) d ∅.
+: set X := of_list (List.map fst (elements d)).
 
-Inductive ge : option val -> option val -> Prop :=
-  | geTop v : ge None (Some v)
-  | geEq v : ge (Some v) (Some v).
-
-Instance ge_dec x y : Computable (ge x y).
-destruct x, y; try dec_solve.
-decide (v = v0); subst; try dec_solve.
-Defined.
-
-
-Instance lt_find_dec d d' x : Computable ((fun x0 : var => ge (find x0 d) (find x0 d')) x).
+Lemma domain_join (d d':Dom)
+: domain (map2 join d d') [=] domain d ∪ domain d'.
 Proof.
-  hnf; intros. eapply ge_dec.
+  unfold domain. split; intros.
+  - eapply of_list_1 in H.
+Admitted.
+
+
+Inductive lt : option (withTop val) -> option (withTop val) -> Prop :=
+  | ltTop v : lt (Some v) (Some Top)
+  | ltBot w : lt None (Some w).
+
+Instance lt_dec x y : Computable (lt x y).
+destruct x, y; try dec_solve.
+destruct w, w0; dec_solve.
 Defined.
 
+Instance lt_find_dec d d' x : Computable ((fun x0 : var => lt (find x0 d) (find x0 d')) x).
+Proof.
+  hnf; intros. eapply lt_dec.
+Defined.
 
-Inductive geDom : Dom -> Dom -> Prop :=
-  | geDomNone d' : geDom (Some d') None
-  | geDomLt (d d':Map [var, val])
-    : (forall x, x ∈ domain d ∪ domain d' -> ge (find x d) (find x d'))
-      -> geDom (Some d) (Some d').
+Definition ltDom (d d': Dom) : Prop :=
+ (forall x, x ∈ domain d ∪ domain d' -> lt (find x d) (find x d')).
 
 Definition set_quant_dec X `{OrderedType X} s P `{Proper _ (_eq ==> iff) P}  `{forall x, Computable (P x) } : bool :=
   SetInterface.fold (fun x b => if [P x] then b else false) s true.
@@ -102,91 +102,172 @@ Defined.
 
 Arguments set_quant_computable [X] {H} s P {H0} {H1}.
 
-Instance geDom_dec
-  :  forall d d' : Dom, Computable (geDom d d').
+Instance ltDom_dec
+  :  forall d d' : Dom, Computable (ltDom d d').
 Proof.
   intros; hnf; intros.
-  destruct d, d'; try dec_solve.
-  edestruct (@set_quant_computable _ _ (domain d ∪ domain d0) (fun x => ge (find x d) (find x d0))); try dec_solve.
+  edestruct (@set_quant_computable _ _ (domain d ∪ domain d') (fun x => lt (find x d) (find x d'))).
   - unfold Proper, respectful; intros.
     hnf in H; subst; intuition.
-  - intros; eapply ge_dec.
+  - intros; eapply lt_dec.
+  - eauto.
+  - right; eauto.
 Defined.
 
-Instance Equal_computable (s t:Map [var, val])
+Instance Equal_computable (s t:Map [var, withTop val])
 : Computable (Equal s t).
-pose (R:=inst_eq_dec_val).
+pose (R:=@withTop_eq_dec _ _ inst_eq_dec_val).
 case_eq (equal R s t); intros.
 eapply MF.equal_iff in H. subst R.
 eapply MF.Equal_Equivb in H. left; eauto.
-intros. destruct (inst_eq_dec_val e e'); intuition.
+intros. destruct (withTop_eq_dec val e e'); intuition.
 right; intro.
 eapply MF.Equal_Equivb in H0.
 eapply MF.equal_iff in H0. instantiate (1:=fun x y => R x y) in H0.
 congruence.
 intros; simpl. subst R.
-destruct (inst_eq_dec_val e e'); intuition.
+destruct (withTop_eq_dec val e e'); intuition.
 Defined.
 
-Definition ltDom d d' := ~ geDom d' d.
-
-Lemma ltDom_dec
-  :  forall d d' : Dom, Computable (ltDom d d').
+Lemma not_domain_find {X} `{OrderedType X} {Y} (d:Map [X, Y]) x
+: x ∉ domain d -> find x d = None.
 Proof.
-  unfold ltDom. intros.
-  decide (geDom d' d).
-  + right. intro. eauto.
-  + left; eauto.
-Defined.
+  unfold domain. intros.
+  case_eq (find x d); intros; eauto.
+  exfalso. eapply H0.
+  rewrite MapFacts.elements_o in H1.
+  Lemma findA_get A B (L:list (A * B)) f v
+  : findA f L = Some v
+    -> exists x n, get L n x /\ snd x = v /\ f (fst x).
+  Proof.
+    general induction L; simpl; eauto.
+    - simpl in H. destruct a. destruct if in H.
+    + inv H.
+      eexists (a,v). eexists 0. repeat split; eauto using get. simpl.
+      rewrite <- Heq. eapply I.
+    + edestruct IHL as [? [? ]]; dcr; eauto.
+      do 2 eexists; eauto using get.
+  Qed.
+  eapply findA_get in H1. destruct H1 as [? [? ]]; dcr; subst.
+  unfold MapFacts.eqb in H5.
+  cbv in H5. destruct x0.
+  pose proof (_compare_spec x x0).
+  Transparent compare. unfold compare in H5.
+  inv H1; rewrite  <- H3 in H5; intuition.
+  rewrite H4.
+  eapply get_in_of_list. change x0 with (fst (x0, y)). eapply map_get_1; eauto.
+Qed.
+
+Lemma domain_find {X} `{OrderedType X} {Y} (d:Map [X, Y]) x
+: x ∈ domain d -> exists v, find x d = Some v.
+Proof.
+  unfold domain.
+  case_eq (find x d); intros; eauto.
+  exfalso.
+  admit.
+Qed.
 
 
-Instance Dom_semilattice : PartialOrder Dom := {
+Lemma lt_join x y x' y'
+: lt y x
+  -> lt y' x'
+  -> lt (join y y') (join x x').
+Proof.
+  intros.
+  inv H; inv H0; simpl; eauto using lt;
+  try destruct v; try destruct v0; try destruct w; eauto using lt.
+  - destruct if; eauto using lt.
+  - destruct w0; eauto. destruct if; eauto using lt.
+Qed.
+
+Lemma join_bot_right (y:Dom) x0
+  : join (find x0 y) ⎣⎦ = find x0 y.
+Proof.
+  destruct (find x0 y); simpl; eauto.
+  destruct w; eauto.
+Qed.
+
+Lemma join_bot_left (y:Dom) x0
+  : join ⎣⎦ (find x0 y) = find x0 y.
+Proof.
+  destruct (find x0 y); simpl; eauto.
+  destruct w; eauto.
+Qed.
+
+Lemma ltDom_join x y x' y'
+: ltDom y x
+  -> ltDom y' x'
+  -> ltDom (joinDom y y') (joinDom x x').
+Proof.
+  unfold ltDom, joinDom.
+  intros.
+  repeat rewrite MapFacts.map2_1bis; eauto.
+  repeat rewrite domain_join in H1.
+  cset_tac.
+  decide (x0 ∈ domain y);
+  decide (x0 ∈ domain y');
+  decide (x0 ∈ domain x);
+  decide (x0 ∈ domain x'); (try now intuition);
+  repeat match goal with
+    | [H' : ?x ∈ domain y |- _ ] => exploit (H x); eauto;
+                                 eapply domain_find in H'; destruct H'
+    | [H' : ?x ∈ domain x |- _ ] => exploit (H x); eauto;
+                                 eapply domain_find in H'; destruct H'
+    | [H' : ?x ∈ domain y' |- _ ] => exploit (H0 x); eauto;
+                                 eapply domain_find in H'; destruct H'
+    | [H' : ?x ∈ domain x' |- _ ] => exploit (H0 x); eauto;
+                                 eapply domain_find in H'; destruct H'
+  end; (try now eapply lt_join; eauto);
+  repeat match goal with
+      | [H' : ?x ∉ domain ?y |- _ ] => eapply not_domain_find in H'; rewrite H'
+         end;
+  repeat rewrite join_bot_right;
+  repeat rewrite join_bot_left; eauto; simpl;
+  repeat match goal with
+    | [H : lt ?x ?y, H' : ?y = None |- _ ] => rewrite H' in H; inv H
+  end.
+  rewrite H2. econstructor.
+  rewrite H2. econstructor.
+Qed.
+
+Set Implicit Arguments.
+
+Instance Dom_semilattice_ltDom : PartialOrder Dom := {
   poLt := ltDom;
   poLt_dec := ltDom_dec;
-  poEq := option_eq Equal;
+  poEq := Equal;
   poEq_dec := _
 }.
-hnf; intros. destruct d,d'; try dec_solve.
-edestruct (Equal_computable d d0); try dec_solve.
-Defined.
 
 Instance set_var_semilattice : BoundedSemiLattice Dom := {
-  bottom := None;
+  bottom := (@empty var _ _ (withTop val));
   join := joinDom
 }.
 - intros. hnf. unfold joinDom.
-  destruct a; eauto using @option_eq.
-  econstructor. hnf; intros.
-  rewrite MapFacts.map2_1bis; unfold join.
-  destruct (find y d); try destruct if; eauto; congruence.
-  congruence.
+  intros.
+  rewrite MapFacts.map2_1bis; unfold join; eauto.
+  destruct (find y a); try destruct if; eauto; try congruence.
+  destruct w; eauto. destruct if; eauto. congruence.
 - hnf; intros. unfold joinDom.
-  destruct a, b; simpl; eauto using @option_eq; try reflexivity.
-  econstructor.
   hnf; intros.
   repeat rewrite MapFacts.map2_1bis; try reflexivity.
-  destruct (find y d), (find y d0); simpl; repeat destruct if; congruence.
+  destruct (find y a), (find y b); simpl; repeat destruct if; try destruct w; try destruct w0; try congruence.
+  repeat destruct if; try subst a0; eauto; try congruence.
 - intros; hnf; intros.
-  destruct a,b,c; simpl; try econstructor; eauto; try reflexivity.
-  hnf; intro.
+  unfold joinDom.
   repeat rewrite MapFacts.map2_1bis; try reflexivity.
-  destruct (find y d), (find y d0), (find y d1); simpl; repeat destruct if; subst; simpl; try congruence.
+  destruct (find y a), (find y b), (find y c); simpl; repeat destruct if; subst; simpl;
+    try destruct w; try destruct w0; try destruct w1; simpl; repeat destruct if; try subst;
+    simpl; try congruence.
   destruct if; congruence.
   destruct if; congruence.
 - unfold Proper, respectful; intros.
   simpl in *.
-  destruct x, y, x0, y0; simpl; eauto using @option_eq; try reflexivity; try eassumption; isabsurd.
-  inv H; inv H0.
-  econstructor.
-  intro. repeat rewrite MapFacts.map2_1bis; try reflexivity.
-  unfold join. rewrite H3. rewrite H4.
+  intro. unfold joinDom. repeat rewrite MapFacts.map2_1bis; try reflexivity.
+  unfold join. rewrite H. rewrite H0.
   reflexivity.
 - unfold Proper, respectful; intros.
-  simpl in *.
-  intro.
-  hnf in H, H0.
-  unfold joinDom in H1.
-  admit.
+  eapply ltDom_join; eauto.
 Qed.
 
 
@@ -229,68 +310,65 @@ Qed.
 
   Fixpoint update_with_list X `{OrderedType X} Y XL YL (m:Map [X, Y]) :=
     match XL, YL with
-      | x::XL, Some y::YL => (update_with_list XL YL m)[x <- y]
-      | x::XL, None::YL => remove x (update_with_list XL YL m)
+      | x::XL, y::YL => (update_with_list XL YL m)[x <- y]
       | _, _ => m
     end.
 
-  Local Notation "f [ w <-- x ]" := (update_with_list w x f) (at level 29, left associativity).
+Local Notation "f [ w <-- x ]" := (update_with_list w x f) (at level 29, left associativity).
 
-Definition defdom (d:Dom) : Map [var, val] :=
-  match d with
-    | Some d => d
-    | None => empty _
+Definition domupd (d:Dom) x (o:option val) : Dom :=
+  match o with
+    | Some xv => (d [x <- wTA xv])
+    | None => (d [x <- Top])
   end.
 
-Definition domupd (d:Map [var, val]) x (o:option val) : Map [var, val] :=
-  match o with
-    | Some xv => (d [x <- xv])
-    | None => (remove x d)
+Definition domenv (d:Dom) (x:var) : option val :=
+  match find x d with
+    | Some (wTA v) => Some v
+    | _ => None
   end.
 
 Definition constant_propagation_transform st (a:list (Dom * params)*Dom) :=
   match st, a with
     | stmtExp x e s as st, (AL, d) =>
-      let d' := (defdom d) in
-      let d'' := domupd d' x (exp_eval (fun x => find x d') e) in
-      (AL, anni1 (Some d''))
+      let d' := d in
+      let d'' := domupd d' x (exp_eval (domenv d') e) in
+      (AL, anni1 d'')
     | stmtIf e s t as st, (AL, d) =>
-      let d := defdom d in
       let ai :=
-          if [exp_eval (fun x => find x d) e = Some val_true] then
+          if [exp_eval (domenv d) e = Some val_true] then
               match e with
-                | BinOp 3 (Var x) (Con c) => anni2opt (Some (Some (d[x <- c]))) None
-                | _ => anni2opt (Some (Some d)) None
+                | BinOp 3 (Var x) (Con c) => anni2opt (Some (d[x <- wTA c])) None
+                | _ => anni2opt (Some d) None
               end
-          else if [exp_eval (fun x => find x d) e = Some val_false] then
+          else if [exp_eval (domenv d) e = Some val_false] then
             match e with
-              | Var x => anni2opt None (Some (Some (d[x <- 0])))
+              | Var x => anni2opt None (Some (d[x <- wTA 0]))
 (*            | BinOp 4 (Var x) (Con c) => anni2opt None (Some (Some (d[x <- c]))) *)
-              | _ => anni2opt None (Some (Some d))
+              | _ => anni2opt None (Some d)
             end
           else
-            anni2opt (Some (Some d)) (Some (Some d))
+            anni2opt (Some d) (Some d)
       in
       (AL, ai)
     | stmtGoto f Y as st, (AL, d) =>
-      let d := defdom d in
       let df := nth (counted f) AL (bottom, nil) in
-      let Yc := List.map (fun e => exp_eval (fun x => find x d) e) Y in
+      let Yc := List.map (fun e => match exp_eval (domenv d) e with
+                        | Some v => wTA v
+                        | None => Top
+                        end ) Y in
       (* we assume renamed apart here, so it's ok to leave definitions
        in d[X <-- Yc] that are /not/ defined at the point where f is defined *)
-      let d' := (Some (d [snd df <-- Yc])) in
+      let d' := (d [snd df <-- Yc]) in
       (list_update_at AL (counted f) (joinDom (fst df) d', snd df), anni1 d')
     | stmtReturn e as st, (AL, d) =>
-      let d := defdom d in
-      (AL, anni1 (Some d))
+      (AL, anni1 d)
     | stmtExtern x f Y s as st, (AL, d) =>
-      let d := defdom d in
       (* we assume renamed apart here, and dont zero x *)
-      (AL, anni1 (Some d))
+      (AL, anni1 d)
     | stmtLet Z s t as st, (AL, d) =>
-      let d' := defdom d in
       (* we assume renamed apart here, and dont zero Z *)
-      (AL, anni2 d (Some d'))
+      (AL, anni2 d d)
   end.
 
 Instance list_equal_computable X `{@EqDec X eq _}
